wip: compute_char_transfer proof

theories/equivalence/StringUtils.v
@@ -29,3 +29,123 @@ Fixpoint has_labeled_instr p_str (lbl : label)  :=
                                        | None => has_labeled_instr t lbl
                                        end
   end.
+
+Lemma has_labeled_instr_app :
+  forall l1 l2 lbl,
+  StringUtils.has_labeled_instr l1 lbl = false ->
+  StringUtils.has_labeled_instr (l1 ++ l2) lbl =
+  StringUtils.has_labeled_instr l2 lbl.
+Proof.
+  induction l1; intros. 
+  - reflexivity.
+  - simpl. destruct a, o; auto.
+    simpl in H. destruct (eqb_lbl lbl l); try discriminate; auto.
+Qed.
+
+Fixpoint labels_greater_than p_str value :=
+  match p_str with
+  | [] => True
+  | StringLang.Instr opt_lbl _ :: t => match opt_lbl with 
+                                       | Some (A n) => n > value 
+                                                       /\
+                                                       labels_greater_than t value
+                                       | None => labels_greater_than t value 
+                                       end
+  end.
+
+Fixpoint labels_less_than p_str value :=
+  match p_str with
+  | [] => True
+  | StringLang.Instr opt_lbl _ :: t => match opt_lbl with 
+                                       | Some (A n) => n < value 
+                                                       /\
+                                                       labels_less_than t value
+                                       | None => labels_less_than t value 
+                                       end
+  end.
+
+
+Lemma labels_greater_implies_diff :
+  forall p_str n value,
+  labels_greater_than p_str value ->
+  n <= value ->
+  has_labeled_instr p_str (A n) = false.
+Proof.
+  induction p_str; intros.
+  + reflexivity.
+  + simpl. simpl in H. destruct a, o.
+    ++ destruct l. assert (n =? n0 = false).
+       { rewrite PeanoNat.Nat.eqb_neq. lia. }
+       rewrite H1. eapply IHp_str; eauto. 
+       destruct H. auto.
+    ++ eapply IHp_str; eauto.
+Qed.
+
+Lemma labels_less_implies_diff :
+  forall p_str n value,
+  labels_less_than p_str value ->
+  n >= value ->
+  has_labeled_instr p_str (A n) = false.
+Proof.
+  induction p_str; intros.
+  + reflexivity.
+  + simpl. simpl in H. destruct a, o.
+    ++ destruct l. assert (n =? n0 = false).
+       { rewrite PeanoNat.Nat.eqb_neq. lia. }
+       rewrite H1. eapply IHp_str; eauto. 
+       destruct H. auto.
+    ++ eapply IHp_str; eauto.
+Qed.
+
+
+Lemma labels_greater_than_app :
+  forall h t value,
+  labels_greater_than h value ->
+  labels_greater_than t value ->
+  labels_greater_than (h ++ t) value.
+Proof.
+  induction h; intros; auto.
+  simpl in *. destruct a. destruct o; auto.
+  destruct l. destruct H. split; auto.
+Qed.
+
+Lemma labels_less_than_app :
+  forall h t value,
+  labels_less_than h value ->
+  labels_less_than t value ->
+  labels_less_than (h ++ t) value.
+Proof.
+  induction h; intros; auto.
+  simpl in *. destruct a. destruct o; auto.
+  destruct l. destruct H. split; auto.
+Qed.
+
+
+Lemma labels_greater_than_S :
+  forall p_str value,
+  labels_greater_than p_str (S value) ->
+  labels_greater_than p_str value.
+Proof.
+  induction p_str; intros; auto.
+  simpl. destruct a, o; auto.
+  destruct l. simpl in H. destruct H. split; auto.
+  lia.
+Qed.
+
+Lemma get_labeled_instr_app :
+  forall l1 l2 lbl,
+  has_labeled_instr l1 lbl = false ->
+  StringLang.get_labeled_instr (l1 ++ l2) lbl
+  =
+  length l1 + StringLang.get_labeled_instr l2 lbl.
+Proof.
+  induction l1; intros.
+  - simpl. reflexivity.
+  - simpl. simpl in H. destruct a eqn:E1. simpl.
+    destruct o.
+    + simpl. rewrite eqb_lbl_symm.
+      destruct (eqb_lbl lbl l).
+      ++ discriminate H. 
+      ++ f_equal. auto.
+    + simpl. f_equal; auto.
+Qed.
